proof/correctness/avx2/KyberPoly_avx2_proof.ec
@@ -2812,44 +2812,39 @@ lemma bit_encode (x: W256.t) (i: int):
   let n = 3 - (i %% 4) in
   let k = ((i %% 32) + n) %/ 16 in
   let sl = W8.of_int (15 - (((i %% 32) + n) %% 16)) in
-    s_encode x.[i] = inzmod (W16.to_sint ((((((x \bits32 di) `<<` (W8.of_int n)) \bits16 k) `<<` sl) `|>>` (W8.of_int 15)) `&` (W16.of_int 1665))).
+    s_encode x.[i] = W16.to_sint ((((((x \bits32 di) `<<` (W8.of_int n)) \bits16 k) `<<` sl) `|>>` (W8.of_int 15)) `&` (W16.of_int 1665)).
 proof.
   move => i_i di n k sl.
-  rewrite /s_encode. rewrite /trueval /falseval.
+  rewrite /s_encode /trueval /falseval.
   have ->: ((q + 1) %/ 2) = 1665.
     rewrite qE. trivial.
 
- have x_msk:
-  forall j, 0 <= j < 16 => (((((x \bits32 di) `<<` (W8.of_int n)) \bits16 k) `<<` sl) `|>>` (W8.of_int 15)).[j]  = x.[i].
-    rewrite /W16.(`|>>`) /sar //=.
-    move => j j_i.
-    rewrite initiE //=.
-    rewrite (_: min 15 (j + 15) = 15); first by smt().
-    rewrite /W16.(`<<`) /W16.(`<<<`).
-    rewrite /sl.
-    rewrite of_uintK.
-    rewrite pmod_small.
-      smt(@W8 @IntDiv @Int).
-    rewrite pmod_small.
-      smt(@W8 @IntDiv @Int).
-    rewrite initiE //=.
-    rewrite (_: 15 - (15 - (i %% 32 + n) %% 16) = (i %% 32 + n) %% 16). smt(@Int).
-    rewrite bits16E /k divzE.
-    rewrite initiE 1:/# //=.
-    rewrite -addzA addNz addz0.
-    rewrite /W32.(`<<`) /W32.(`<<<`).
-    rewrite initiE 1:/# //=.
-    rewrite (pmod_small n).
-      by smt(@IntDiv @Int).
-    rewrite (pmod_small n).
-      by smt(@IntDiv @Int).
-    rewrite -(addzA _ n) addzN addz0.
-    rewrite bits32E /di divzE.
-    rewrite initiE 1:/# //=.
-    rewrite -addzA addNz addz0 //=.
+  have x_msk:
+    forall j, 0 <= j < 16 => (((((x \bits32 di) `<<` (W8.of_int n)) \bits16 k) `<<` sl) `|>>` (W8.of_int 15)).[j]  = x.[i].
+      rewrite /W16.(`|>>`) /sar //=.
+      move => j j_i.
+      rewrite initiE //=.
+      rewrite (_: min 15 (j + 15) = 15); first by smt().
+      rewrite /W16.(`<<`) /W16.(`<<<`).
+      rewrite /sl.
+      rewrite of_uintK.
+      rewrite pmod_small. by smt(@W8 @IntDiv @Int).
+      rewrite pmod_small. by smt(@W8 @IntDiv @Int).
+      rewrite initiE //=.
+      rewrite (_: 15 - (15 - (i %% 32 + n) %% 16) = (i %% 32 + n) %% 16). smt(@Int).
+      rewrite bits16E /k divzE.
+      rewrite initiE 1:/# //=.
+      rewrite -addzA addNz addz0.
+      rewrite /W32.(`<<`) /W32.(`<<<`).
+      rewrite initiE 1:/# //=.
+      rewrite (pmod_small n). by smt(@IntDiv @Int).
+      rewrite (pmod_small n). by smt(@IntDiv @Int).
+      rewrite -(addzA _ n) addzN addz0.
+      rewrite bits32E /di divzE.
+      rewrite initiE 1:/# //=.
+      rewrite -addzA addNz addz0 //=.
 
   case x.[i] => x_i_1.
-  congr.
   have ->: ((((x \bits32 di) `<<` (of_int n)%W8 \bits16 k) `<<` sl) `|>>` (of_int 15)%W8) = W16.onew.
     rewrite wordP. move => j j_i.
     rewrite (x_msk j j_i).
@@ -2858,7 +2853,6 @@ proof.
   rewrite W16.and1w of_sintK /smod //=.
 
   move : x_i_1 => x_i_0.
-  congr.
   have ->: ((((x \bits32 di) `<<` (of_int n)%W8 \bits16 k) `<<` sl) `|>>` (of_int 15)%W8) = W16.zero.
     rewrite wordP. move => j j_i.
     rewrite (x_msk j j_i).
@@ -2875,14 +2869,22 @@ lemma poly_frommsg_corr_h _a:
             lift_array256 res = m_encode _a].
 proof.
   proc.
-  seq 3 : (#pre /\
+
+  seq 4 : (#pre /\
+           (forall k, 0 <= k < 256 => f.[k] = f_dw.[k %/ 32].[k %% 32]) /\
            (forall k, 0 <= k < 16 => hqs.[k] = (W16.of_int 1665)) /\
            (forall k, 0 <= k < 32 => idx.[k] = pfm_idx_s.[k %% 16]) /\
-           (forall k, 0 <= k < 8 => shift.[k] = pfm_shift_s.[k %% 4])).
+           (forall k, 0 <= k < 8 => shift.[k] = W32.of_int (3 - k %% 4))).
   inline *.
   wp. skip.
   move => &hr [#] _a_def pfm_idx_vdef pfm_shift_vdef.
   split; first by rewrite _a_def.
+
+  split.
+  move => k k_i.
+  rewrite initiE 1:/# //=.
+  rewrite bits32E initiE 1:/# /=.
+  rewrite -divz_eq //=.
 
   split.
   move => k k_i.
@@ -2901,28 +2903,486 @@ proof.
 
   split.
   move => k k_i.
-  do rewrite get_setE //.
+  do (rewrite Array32.get_setE //).
   rewrite /pfm_idx_vdef Array16.initiE //=.
   rewrite /(KyberCPA_avx2.pfm_idx_s) initiE //= 1:/#.
   smt(@Array32 @Array16 @IntDiv).
 
   move => k k_i.
-  do rewrite get_setE //.
+  do (rewrite Array8.get_setE //).
   rewrite /pfm_shift_vdef Array4.initiE //=.
-  rewrite /(KyberCPA_avx2.pfm_shift_s) initiE //= 1:/#.
   smt(@Array8 @Array4 @IntDiv).
 
   while(#pre /\
         0 <= i <= 4 /\
-        (forall k, 0 <= k < 32 * i => inzmod (W16.to_sint rp.[k]) = s_encode _a.[k]) /\
-        (forall k, 128 <= k < 128 + 32 * i => inzmod (W16.to_sint rp.[k]) = s_encode _a.[k])).
+        (forall k, 0 <= k < 32 * i => W16.to_sint rp.[k] = s_encode _a.[k]) /\
+        (forall k, 128 <= k < 128 + 32 * i => W16.to_sint rp.[k] = s_encode _a.[k])).
+
+  seq 16: (#pre /\
+           (forall k, 0 <= k < 16 => W16.to_sint g0.[k] = s_encode _a.[32 * i + 128 * (k %/ 8) + 16 * (k %% 8 %/ 4) + (k %% 4)]) /\
+           (forall k, 0 <= k < 16 => W16.to_sint g1.[k] = s_encode _a.[32 * i + 128 * (k %/ 8) + 16 * (k %% 8 %/ 4) + (k %% 4) + 4]) /\
+           (forall k, 0 <= k < 16 => W16.to_sint g2.[k] = s_encode _a.[32 * i + 128 * (k %/ 8) + 16 * (k %% 8 %/ 4) + (k %% 4) + 8]) /\
+           (forall k, 0 <= k < 16 => W16.to_sint g3.[k] = s_encode _a.[32 * i + 128 * (k %/ 8) + 16 * (k %% 8 %/ 4) + (k %% 4) + 12])).
 
   inline *.
   wp. skip.
   simplify.
-  move => &hr [#] *.
+  move => &hr [#] _a_def f_def hqs_def pfm_idx_vdef pfm_shift_vdef i_lb i_ub rpl_def rph_def i_tub.
+  rewrite _a_def i_lb i_ub //=.
 
+  have idx_in_bound: forall k, 0 <= k < 32 => ! 128 <= to_uint idx{hr}.[k].
+    move => k k_i.
+    rewrite (pfm_idx_vdef k k_i).
+    rewrite /(KyberCPA_avx2.pfm_idx_s) initiE //= 1:/#.
+    do (rewrite (fun_if W8.to_uint) //=).
+    smt(@Int @Array16 @IntDiv).
 
+  do split.
+  apply f_def.
+  apply hqs_def.
+  apply pfm_idx_vdef.
+  apply pfm_shift_vdef.
+  apply rpl_def.
+  apply rph_def.
+  apply i_tub.  
+  
+  move => k k_i.
+  do (rewrite initiE 1://= //=).
+  rewrite hqs_def 1://=.
+  rewrite (pmod_small _ 256).
+    move : i_lb i_tub => /#.
+
+  rewrite /f8u32_t32u8 //=.
+  rewrite (_: (Array8.init (fun (i1: int) => ((Array8.init (fun (i2 : int) => f_dw{hr}.[4 * (i2 %/ 4) + 85 * i{hr} %/ (2 ^ (2 * (i2 %% 4))) %% 4]))).[i1] `<<<` to_uint shift{hr}.[i1])) =
+              (Array8.init (fun (i1: int) => f_dw{hr}.[4 * (i1 %/ 4) + 85 * i{hr} %/ (2 ^ (2 * (i1 %% 4))) %% 4] `<<<` to_uint shift{hr}.[i1]))).
+    apply Array8.ext_eq.
+    move => x x_i.
+    do rewrite initiE //=.
+
+  rewrite (_: (Array32.init (fun (i0: int) => (Array8.init (fun (i1 : int) =>
+                                              f_dw{hr}.[4 * (i1 %/ 4) + 85 * i{hr} %/ (2 ^ (2 * (i1 %% 4))) %% 4] `<<<` to_uint shift{hr}.[i1])).[i0 %/ 4] \bits8 i0 %% 4)) =
+              (Array32.init (fun (i0 : int) => (f_dw{hr}.[4 * (i0 %/ 4 %/ 4) + 85 * i{hr} %/ (2 ^ (2 * ((i0 %/ 4) %% 4))) %% 4] `<<<` to_uint shift{hr}.[i0 %/ 4]) \bits8 i0 %% 4))).
+    apply Array32.ext_eq.
+    move => x x_i.
+    do rewrite initiE //=.
+      move : x_i => /#.
+  pose tmp := (Array32.init (fun (i0 : int) => f_dw{hr}.[4 * (i0 %/ 4 %/ 4) + 85 * i{hr} %/ (2 ^ (2 * (i0 %/ 4 %% 4))) %% 4] `<<<`
+                                                to_uint shift{hr}.[i0 %/ 4] \bits8 i0 %% 4)).
+  rewrite (_: (Array32.init (fun (i : int) => if 128 <= to_uint idx{hr}.[i] then W8.zero
+                                               else tmp.[16 * (i %/ 16) + to_uint idx{hr}.[i] %% 16])) =
+               (Array32.init (fun (i: int) => tmp.[16 * (i %/ 16) + to_uint idx{hr}.[i] %% 16]))).
+    apply Array32.ext_eq.
+    move => x x_i.
+    rewrite initiE //=.
+    rewrite (idx_in_bound x x_i) //=.
+    rewrite (Array32.initiE _ x) //=.
+
+  rewrite (_: (W2u8.Pack.init (fun (j: int) => (Array32.init (fun (i : int) =>
+                                                tmp.[16 * (i %/ 16) + to_uint idx{hr}.[i] %% 16])).[2 * k + j])) =
+               W2u8.Pack.init (fun j => tmp.[16 * ((2 * k + j) %/ 16) + to_uint idx{hr}.[2 * k + j]])).
+    apply W2u8.Pack.ext_eq.
+    move => x x_i.
+    do 2!(rewrite initiE 1:/# //=).
+    rewrite W2u8.Pack.initiE 1://= //=.
+    rewrite pmod_small.
+      rewrite pfm_idx_vdef 1:/# /(KyberCPA_avx2.pfm_idx_s) initiE //= 1:/#.
+      do (rewrite (fun_if W8.to_uint) //=).
+      smt(@Int @Array16 @IntDiv @Int).
+    trivial.
+    rewrite (_: W2u8.Pack.init (fun (j : int) => tmp.[16 * ((2 * k + j) %/ 16) + to_uint idx{hr}.[2 * k + j]]) =
+                W2u8.Pack.init (fun (j : int) => f_dw{hr}.[4 * ((16 * ((2 * k + j) %/ 16) + to_uint idx{hr}.[2 * k + j]) %/ 4 %/ 4) + 85 * i{hr} %/ (2 ^ (2 * ((16 * ((2 * k + j) %/ 16) + W8.to_uint idx{hr}.[2 * k + j]) %/ 4 %% 4))) %% 4] `<<<`
+                                                 W32.to_uint shift{hr}.[(16 * ((2 * k + j) %/ 16) + W8.to_uint idx{hr}.[2 * k + j]) %/ 4]
+                                                 \bits8  (16 * ((2 * k + j) %/ 16) + W8.to_uint idx{hr}.[2 * k + j]) %% 4)).
+    apply W2u8.Pack.ext_eq.
+    move => x x_i.
+    rewrite initiE //=.
+    rewrite initiE //=.
+      rewrite pfm_idx_vdef 1:/# /(KyberCPA_avx2.pfm_idx_s) initiE //= 1:/#.
+      do (rewrite (fun_if W8.to_uint) //=).
+      move : x_i k_i => /#.
+    rewrite initiE //=.
+
+  rewrite (_: W2u8.Pack.init (fun (j : int) => f_dw{hr}.[4 * ((16 * ((2 * k + j) %/ 16) + to_uint idx{hr}.[2 * k + j]) %/ 4 %/ 4) +
+                                                         85 * i{hr} %/ (2 ^ (2 * ((16 * ((2 * k + j) %/ 16) +
+                                                         W8.to_uint idx{hr}.[2 * k + j]) %/ 4 %% 4))) %% 4] `<<<`
+                                               W32.to_uint shift{hr}.[(16 * ((2 * k + j) %/ 16) + W8.to_uint idx{hr}.[2 * k + j]) %/ 4]
+                                               \bits8  (16 * ((2 * k + j) %/ 16) + W8.to_uint idx{hr}.[2 * k + j]) %% 4) =
+              W2u8.Pack.init (fun (j : int) => f_dw{hr}.[4 * ((2 * k + j) %/ 16) +
+                                                         85 * i{hr} %/ (2 ^ (2 * (W8.to_uint idx{hr}.[2 * k + j] %/ 4))) %% 4] `<<<`
+                                               W32.to_uint shift{hr}.[(16 * ((2 * k + j) %/ 16) + W8.to_uint idx{hr}.[2 * k + j]) %/ 4]
+                                               \bits8  (16 * ((2 * k + j) %/ 16) + W8.to_uint idx{hr}.[2 * k + j]) %% 4)).
+    apply W2u8.Pack.ext_eq.
+    move => x x_i.
+    rewrite initiE //=.
+    rewrite initiE //=.
+    have idx_bnds: forall w, 0 <= w < 32 => 0 <= to_uint idx{hr}.[w] %/4 && to_uint idx{hr}.[w] %/ 4 < 4.
+      move => w w_i.
+      rewrite pfm_idx_vdef 1:/#.
+      rewrite /(KyberCPA_avx2.pfm_idx_s) initiE //= 1:/#.
+      do (rewrite (fun_if W8.to_uint) //=).
+      smt(@Int @Array16 @IntDiv).
+    rewrite (_: (16 * ((2 * k + x) %/ 16) + to_uint idx{hr}.[2 * k + x]) %/ 4 %% 4 =
+                to_uint idx{hr}.[2 * k + x] %/ 4).
+      move : (idx_bnds (2 * k + x)).
+      smt(@Int @IntDiv).
+    rewrite (_: (16 * ((2 * k + x) %/ 16) + to_uint idx{hr}.[2 * k + x]) %/ 4 %/ 4 =
+                (2 * k + x) %/ 16).
+      move : (idx_bnds (2 * k + x)).
+      smt(@Int @IntDiv).
+    trivial.
+
+  have f_dw_idx : forall j, 0 <= j < 2 => 4 * ((2 * k + j) %/ 16) + 85 * i{hr} %/ (2 ^ (2 * (W8.to_uint idx{hr}.[2 * k + j] %/ 4))) %% 4 =
+                                          4 * (k %/ 8) + i{hr}.
+    move => j j_i.
+    rewrite pfm_idx_vdef 1:/#.
+    move : j_i.
+    rewrite andabP => /(mem_iota 0 2 j).
+    move : k_i.
+    rewrite andabP => /(mem_iota 0 16 k).
+    have i_i: i{hr} \in iota_ 0 4.
+      move : i_lb i_tub.
+      smt(@Int @List).
+    move : i_i.
+    rewrite /(KyberCPA_avx2.pfm_idx_s) initiE //= 1:/#.
+    do (rewrite (fun_if W8.to_uint) //=).
+    move => i_i k_i j_i.
+    admit. (*FIXME : smt(@List @Int @Ring.IntID @IntDiv). *)
+
+  have shift_idx: forall j, 0 <= j < 2 => (16 * ((2 * k + j) %/ 16) + W8.to_uint idx{hr}.[2 * k + j]) %/ 4 = 4 * (k %/ 8) + k %% 4.
+    move => j j_i.
+    rewrite pfm_idx_vdef 1:/#.
+    move : j_i.
+    rewrite andabP => /(mem_iota 0 2 j).
+    move : k_i.
+    rewrite andabP => /(mem_iota 0 16 k).
+    rewrite /(KyberCPA_avx2.pfm_idx_s) initiE //= 1:/#.
+    do (rewrite (fun_if W8.to_uint) //=).
+    move => k_i j_i.
+    admit. (*FIXME : smt(@List @Int @IntExtra @Int @IntDiv). *)
+
+  have bit_idx : forall j, 0 <= j < 2 => (16 * ((2 * k + j) %/ 16) + W8.to_uint idx{hr}.[2 * k + j]) %% 4 = 2 * (k %% 8 %/ 4) + j.
+    move => j j_i.
+    rewrite pfm_idx_vdef 1:/#.
+    move : j_i.
+    rewrite andabP => /(mem_iota 0 2 j).
+    move : k_i.
+    rewrite andabP => /(mem_iota 0 16 k).
+    rewrite /(KyberCPA_avx2.pfm_idx_s) initiE //= 1:/#.
+    do (rewrite (fun_if W8.to_uint) //=).
+    move => k_i j_i.
+    admit. (*FIXME : smt(@List @Int @IntExtra @Int @IntDiv). *)
+
+  rewrite (_: W2u8.Pack.init (fun (j : int) =>
+                              f_dw{hr}.[4 * ((2 * k + j) %/ 16) + 85 * i{hr} %/ (2 ^ (2 * (W8.to_uint idx{hr}.[2 * k + j] %/ 4))) %% 4] `<<<`
+                              to_uint shift{hr}.[(16 * ((2 * k + j) %/ 16) + to_uint idx{hr}.[2 * k + j]) %/ 4] \bits8
+                              (16 * ((2 * k + j) %/ 16) + to_uint idx{hr}.[2 * k + j]) %% 4) =
+              W2u8.Pack.init (fun (j: int) => 
+                              f_dw{hr}.[4 * (k %/ 8) + i{hr}] `<<<`
+                              to_uint shift{hr}.[4 *(k %/ 8) + k %% 4] \bits8 2 * (k %% 8 %/ 4) + j)).
+    apply W2u8.Pack.ext_eq.
+    move => x x_i.
+    do (rewrite initiE //=).
+    rewrite f_dw_idx 1:// shift_idx 1://= bit_idx 1://=.
+    trivial.
+
+  rewrite (_: (pack2_t (W2u8.Pack.init (fun (j: int) => 
+                                f_dw{hr}.[4 * (k %/ 8) + i{hr}] `<<<`
+                                to_uint shift{hr}.[4 *(k %/ 8) + k %% 4] \bits8 2 * (k %% 8 %/ 4) + j)))
+               = f_dw{hr}.[4 * (k %/ 8) + i{hr}] `<<<` to_uint shift{hr}.[4 *(k %/ 8) + k %% 4] \bits16 (k %% 8 %/ 4)).
+    rewrite /pack2_t.
+    rewrite W16.wordP.
+    move => i i_i.
+    rewrite initiE //= initiE 1:/# //=.
+    rewrite bits8E bits16E.
+    rewrite initiE //= initiE 1:/# //=.
+    smt(@Int @IntDiv).
+
+  rewrite (_: f_dw{hr}.[4 * (k %/ 8) + i{hr}] = f{hr} \bits32 (4 * (k %/ 8) + i{hr})).
+    rewrite W32.wordP.
+    move => i i_i.
+    rewrite bits32E.
+    rewrite initiE //=.
+    rewrite f_def 1:/#.
+    smt(@IntDiv).
+
+  pose idx := 32 * i{hr} + 128 * (k %/ 8) + 16 * (k %% 8 %/ 4) + k %% 4.
+  have ->: 4 * (k %/ 8) + i{hr} = idx %/ 32. by smt(@Int @IntDiv).
+
+  rewrite pfm_shift_vdef 1:/# //=.
+  rewrite (mulzC 4 _) modzMDl modz_mod.
+  rewrite of_uintK pmod_small 1:/#.
+
+  have ->: 3 - k %% 4 = 3 - idx %% 4. by smt(@Int @IntDiv).
+  have ->: k %% 8 %/ 4 = (idx %% 32 + (3 - idx %% 4)) %/ 16. by smt(@Int @IntDiv).
+  have ->: 12 = 15 - ((idx %% 32 + (3 - idx %% 4)) %% 16). by smt(@Int @IntDiv).
+
+  pose di := idx %/ 32. 
+  pose n := 3 - idx %% 4.
+  pose kb := (idx %% 32 + n) %/ 16.
+  pose sl := W8.of_int (15 - (idx %% 32 + n) %% 16).
+
+  rewrite -W32.shl_shlw 1:/#.
+  rewrite -_a_def /lift_msg initiE //= 1:/#.
+  move : (bit_encode f{hr} idx).
+  rewrite (_: (0 <= idx && idx < 256) = true) //=. move : k_i i_lb i_tub => /#.
+  rewrite -/di -/n -/kb -/sl.
+  smt(@Logic).
+
+  admit. (* FIXME: same as previous block  *)
+  admit. (* FIXME: same as previous block  *)
+  admit. (* FIXME: same as previous block  *)
+
+  inline *. wp. skip.
+  move => &hr [#] _a_def f_def hqs_def pfm_idx_vdef pfm_shift_vdef i_lb i_ub rpl_def rph_def i_tub g0_def g1_def g2_def g3_def h0_def h2_def h1_def h3_def h0_h1_32 h0_h1_49 h2_h3_32 h2_h3_49 rp_fdef iu.
+  simplify.
+  do split; first 7 by smt().
+
+  move => k k_i.
+  rewrite /rp_fdef.
+  do rewrite filliE 1:/# //=.
+  do (rewrite (fun_if W16.to_sint)).
+
+  have ->: !(144 + 32 * i{hr} <= k && k < 160 + 32 * i{hr}). by move : k_i => /#.
+  have ->: !(128 + 32 * i{hr} <= k && k < 144 + 32 * i{hr}). by move : k_i => /#.
+
+  simplify.
+  do (rewrite initiE 1:/# //=).
+  do (rewrite (fun_if Array16."_.[_]") || rewrite if_arg).
+  do (rewrite (fun_if W16.to_sint)).
+  rewrite /h0_def /h1_def /h2_def /h3_def.
+  do (rewrite initiE 1:/# //=).
+  do (rewrite (fun_if W16.to_sint)).
+
+  rewrite /h0_h1_32 /h2_h3_32.
+
+  have true_32: forall x, 0 <= x < 8 => (W8.of_int 32).[x] = (x = 5).
+    move => x x_i.
+    rewrite get_to_uint x_i of_uintK //=.
+    move : x_i.
+    rewrite andabP => /(mem_iota 0 8 x).
+    move => x_i.
+    admit. (* FIXME *)
+
+  have ->: !(W8.of_int 32).[4 * (k %% 16 %/ 8) + 3].
+    rewrite true_32 1:/#.
+    have k_vals: 0 <= k %% 16 %/ 8 < 2.
+      move : (modz_cmp k 16) => /#.
+    move : k_vals => /#.
+
+  have ->: !(W8.of_int 32).[4 * (k %% 16 %/ 8)].
+    rewrite true_32 1:/#.
+    move : (modz_cmp k 16) => /#.
+
+  simplify.
+
+  rewrite g0_def.
+    rewrite modz_dvd 1://=.
+    rewrite (pdiv_small (k %% 8) 8). by smt(@IntDiv @Int).
+    rewrite modz_dvd 1://=.
+    smt(@IntDiv @Int).
+
+  rewrite g1_def.
+    rewrite modz_dvd 1://=.
+    rewrite (pdiv_small (k %% 8) 8). by smt(@IntDiv @Int).
+    rewrite modz_dvd 1://=.
+    smt(@IntDiv @Int).
+
+  rewrite g2_def.
+    rewrite modz_dvd 1://=.
+    rewrite (pdiv_small (k %% 8) 8). by smt(@IntDiv @Int).
+    rewrite modz_dvd 1://=.
+    smt(@IntDiv @Int).
+
+  rewrite g3_def.
+    rewrite modz_dvd 1://=.
+    rewrite (pdiv_small (k %% 8) 8). by smt(@IntDiv @Int).
+    rewrite modz_dvd 1://=.
+    smt(@IntDiv @Int).
+
+  rewrite g0_def.
+    move : (modz_cmp k 4) => /#.
+  rewrite g1_def.
+    move : (modz_cmp k 4) => /#.
+  rewrite g2_def.
+    move : (modz_cmp k 4) => /#.
+  rewrite g3_def.
+    move : (modz_cmp k 4) => /#.
+
+  do (rewrite modz_dvd 1://=).
+  rewrite (pdiv_small (k %% 8) 8). by smt(@IntDiv @Int).
+  rewrite (_: ((4 + k %% 4) %% 8 %/ 4) = 1). by smt(@IntDiv @Int).
+  rewrite (_: ((4 + k %% 4) %/ 8) = 0). by smt(@IntDiv @Int).
+  rewrite (_: ((4 + k %% 4) %% 4) = k %% 4). by smt(@IntDiv @Int).  
+  rewrite (_: k %% 8 %/ 4 %% 2 = k %/ 4 %% 2). by smt(@IntDiv @Int @Ring.IntID).
+  rewrite (_: k %% 4 %% 8 %/ 4 = 0). by smt(@IntDiv @Int).
+  rewrite (pdiv_small (k %% 4) 8). by smt(@IntDiv @Int).
+  simplify.
+  rewrite modz_mod.  
+
+  rewrite (_: (0 <= 4 * (k %% 16 %/ 8) + 1 && 4 * (k %% 16 %/ 8) + 1 < 8) = true) //=.
+    by smt(@IntDiv @Int).
+
+  case (32 * i{hr} + 16 <= k && k < 32 * i{hr} + 32)  => k_ssi.
+    case (32 * i{hr} + 24 <= k && k < 32 * i{hr} + 32) => k_sssi.
+      have ->: W8.int_bit 32 (4 * (k %% 16 %/ 8) + 1).
+        move : (true_32 (4 * (k %% 16 %/ 8) + 1)).
+        smt(@W8 @Int @IntDiv).
+      simplify.
+      smt(@Int @IntDiv @W16 @Array256 @Logic @List).
+      have ->: !W8.int_bit 32 (4 * (k %% 16 %/ 8) + 1).
+          move : (true_32 (4 * (k %% 16 %/ 8) + 1)).
+        smt(@W8 @Int @IntDiv).
+      simplify.
+      smt(@Int @IntDiv @W16 @Array256 @Logic @List).
+  move : k_ssi => k_nssi.
+  case (32 * i{hr} <= k && k < 32 * i{hr} + 16)  => k_ssi.
+    case (32 * i{hr} + 8 <= k && k < 32 * i{hr} + 16) => k_sssi.
+      have ->: W8.int_bit 32 (4 * (k %% 16 %/ 8) + 1).
+        move : (true_32 (4 * (k %% 16 %/ 8) + 1)).
+        smt(@W8 @Int @IntDiv).
+      simplify.
+      smt(@Int @IntDiv @W16 @Array256 @Logic @List).
+      have ->: !W8.int_bit 32 (4 * (k %% 16 %/ 8) + 1).
+          move : (true_32 (4 * (k %% 16 %/ 8) + 1)).
+        smt(@W8 @Int @IntDiv).
+      simplify.
+      smt(@Int @IntDiv @W16 @Array256 @Logic @List).
+  apply rpl_def.
+  move : k_nssi k_ssi k_i => /#.
+
+  move => k k_i.
+  rewrite /rp_fdef.
+  do rewrite filliE 1:/# //=.
+  do (rewrite (fun_if W16.to_sint)).
+
+  have ->: !(32 * i{hr} + 16 <= k && k < 32 * i{hr} + 32). by move : k_i => /#.
+  have ->: !(32 * i{hr} <= k && k < 32 * i{hr} + 16). by move : k_i => /#.
+
+  simplify.
+  do (rewrite initiE 1:/# //=).
+  do (rewrite (fun_if Array16."_.[_]") || rewrite if_arg).
+  do (rewrite (fun_if W16.to_sint)).
+  rewrite /h0_def /h1_def /h2_def /h3_def.
+  do (rewrite initiE 1:/# //=).
+  do (rewrite (fun_if W16.to_sint)).
+
+  rewrite /h0_h1_49 /h2_h3_49.
+
+  have true_49: forall x, 0 <= x < 8 => (W8.of_int 49).[x] = (x = 5 \/ x = 4 \/ x = 0).
+    move => x x_i.
+    rewrite get_to_uint x_i of_uintK //=.
+    move : x_i.
+    rewrite andabP => /(mem_iota 0 8 x).
+    move => x_i.
+    admit. (* FIXME *)
+
+  have ->: !(W8.of_int 49).[4 * (k %% 16 %/ 8) + 3].
+    rewrite true_49 1:/#.
+    move : (modz_cmp k 16) => /#.
+
+  simplify.
+
+  do (rewrite modz_dvd 1://=).
+  rewrite (_: (8 + k %% 8) %/ 8 = 1). by smt(@IntDiv @Int).
+  rewrite (_: (8 + k %% 8) %/ 4 %% 2 = k %/ 4 %% 2). by smt(@IntDiv @Int).
+  rewrite (_: k %% 8 %/ 4 %% 2 = k %/ 4 %% 2). by smt(@IntDiv @Int @Ring.IntID).
+  rewrite (_: (8 + k %% 8) %% 4 = k %% 4). by smt(@IntDiv @Int).
+  rewrite (pdiv_small (k %% 8) 8). by smt(@IntDiv @Int).
+  have ->: 0 <= 4 * (k %% 16 %/ 8) && 4 * (k %% 16 %/ 8) < 8. by smt(@IntDiv @Int).
+  have ->: 0 <= 4 * (k %% 16 %/ 8) + 1 && 4 * (k %% 16 %/ 8) + 1 < 8. by smt(@IntDiv @Int).
+  simplify.
+
+  do (rewrite g0_def; first by move : (modz_cmp k 4) => /#).
+  do (rewrite g1_def; first by move : (modz_cmp k 4) => /#).
+  do (rewrite g2_def; first by move : (modz_cmp k 4) => /#).
+  do (rewrite g3_def; first by move : (modz_cmp k 4) => /#).
+
+  rewrite (_: (12 + k %% 4) %/ 8 = 1). by smt(@IntDiv @Int).
+  rewrite (_: (12 + k %% 4) %% 8 %/ 4 = 1). by smt(@IntDiv @Int).
+  rewrite (_: (12 + k %% 4) %% 4 = k %% 4). by smt(@IntDiv @Int).
+  rewrite (_: (8 + k %% 4) %/ 8 = 1). by smt(@IntDiv @Int).
+  rewrite (_: (8 + k %% 4) %% 8 %/ 4 = 0). by smt(@IntDiv @Int).
+  rewrite (_: (8 + k %% 4) %% 4 = k %% 4). by smt(@IntDiv @Int).
+  rewrite (_: ((4 + k %% 4) %% 8 %/ 4) = 1). by smt(@IntDiv @Int).
+  rewrite (_: ((4 + k %% 4) %/ 8) = 0). by smt(@IntDiv @Int).
+  rewrite (_: ((4 + k %% 4) %% 4) = k %% 4). by smt(@IntDiv @Int).
+  rewrite (pdiv_small (k %% 4) 8). by smt(@IntDiv @Int).
+  rewrite (pdiv_small (k %% 4 %% 8) 4). by smt(@IntDiv @Int).
+  rewrite modz_mod.
+  simplify.
+
+  case (144 + 32 * i{hr} <= k && k < 160 + 32 * i{hr}) => k_si.
+    case (152 + 32 * i{hr} <= k && k < 160 + 32 * i{hr}) => k_ssi.
+      have ->: W8.int_bit 49 (4 * (k %% 16 %/ 8)).
+        move : (true_49 (4 * (k %% 16 %/ 8))).
+        smt(@W8 @Int @IntDiv).
+      have ->: W8.int_bit 49 (4 * (k %% 16 %/ 8) + 1).
+        move : (true_49 (4 * (k %% 16 %/ 8))).
+        smt(@W8 @Int @IntDiv).
+      simplify.
+      smt(@Int @IntDiv @W16 @Array256 @Logic @List).
+      have ->: W8.int_bit 49 (4 * (k %% 16 %/ 8)).
+        move : (true_49 (4 * (k %% 16 %/ 8))).
+        smt(@W8 @Int @IntDiv).
+      have ->: !W8.int_bit 49 (4 * (k %% 16 %/ 8) + 1).
+        move : (true_49 (4 * (k %% 16 %/ 8) + 1)).
+        smt(@W8 @Int @IntDiv).
+      smt(@Int @IntDiv @W16 @Array256 @Logic @List).
+  move : k_si => k_nsi.
+  case (128 + 32 * i{hr} <= k && k < 144 + 32 * i{hr})  => k_si.
+    case (136 + 32 * i{hr} <= k && k < 144 + 32 * i{hr})  => k_ssi.
+      have ->: W8.int_bit 49 (4 * (k %% 16 %/ 8)).
+        move : (true_49 (4 * (k %% 16 %/ 8))).
+        smt(@W8 @Int @IntDiv).
+      have ->: W8.int_bit 49 (4 * (k %% 16 %/ 8) + 1).
+        move : (true_49 (4 * (k %% 16 %/ 8))).
+        smt(@W8 @Int @IntDiv).
+      simplify.
+      smt(@Int @IntDiv @W16 @Array256 @Logic @List).
+      have ->: W8.int_bit 49 (4 * (k %% 16 %/ 8)).
+        move : (true_49 (4 * (k %% 16 %/ 8))).
+        smt(@W8 @Int @IntDiv).
+      have ->: !W8.int_bit 49 (4 * (k %% 16 %/ 8) + 1).
+        move : (true_49 (4 * (k %% 16 %/ 8) + 1)).
+        smt(@W8 @Int @IntDiv).
+      smt(@Int @IntDiv @W16 @Array256 @Logic @List).
+  apply rph_def.
+  move : k_nsi k_si k_i => /#.
+
+  sp. skip. simplify.
+  move => &hr [#] i_val _a_def f_def hqs_def pfm_idx_vdef pfm_shift_vdef.
+  do split; first 5 by smt().
+  rewrite i_val => /#.
+  rewrite i_val => /#.
+  rewrite i_val => /#.
+  rewrite i_val => /#.
+
+  move => [#] i rp i_tlb [#] _a_ddef f_ddef hqs_ddef pfm_idx_dvdef pfm_shift_dvdef i_lb i_ub.
+  have i_nval: i = 4. by move : i_ub i_tlb => /#.
+  rewrite i_nval //=.
+  move => rpl_def rph_def.
+
+  have rp_def: map W16.to_sint rp = map s_encode _a.
+    rewrite /s_encode.
+    apply Array256.ext_eq.
+    move => x x_i.
+    do (rewrite Array256.mapiE 1:x_i //=).
+    move : rpl_def rph_def => /#.
+
+  split.
+  rewrite /pos_bound256_cxq /bpos16.
+  move => k k_i /=.
+  move : rp_def => /#.
+
+  rewrite /lift_array256 /m_encode.
+  apply Array256.ext_eq => x x_i.
+  do rewrite mapiE //=.
+
+  rewrite Array256.tP in rp_def.
+  move : (rp_def x x_i).
+  do rewrite mapiE //=.
+  rewrite /s_encode.
+  smt(@Array256 @W16 @Int @ZModField).
 qed.
 
 
